src/tc/tc.fs
@@ -314,6 +314,8 @@ and tc_typ env (t:typ) : typ * knd * guard_t =
  
   | Typ_refine(x, phi) -> 
     let x, env, f1 = tc_vbinder env x in 
+    if debug env Options.High then Util.fprint3 "(%s) Checking refinement formula %s; env expects type %s\n"  (Range.string_of_range top.pos) (Print.typ_to_string phi) (match Env.expected_typ env with None -> "None" | Some t -> Print.typ_to_string t);
+       
     let phi, f2 = tc_typ_check env phi ktype in
     w ktype <| mk_Typ_refine(x, phi), ktype, Rel.conj_guard f1 (Rel.close_guard [v_binder x] f2)
 
@@ -588,6 +590,7 @@ and tc_value env e : exp * lcomp * guard_t =
                  let mk_letrec_environment actuals env = match env.letrecs with 
                     | [] -> env
                     | letrecs ->
+                     let _ = if Tc.Env.debug env Options.High then Util.fprint1 "Building let-rec environment... type of this abstraction is %s\n" (Print.typ_to_string t) in
                      let r = Env.get_range env in
                      let env = {env with letrecs=[]} in 
                    
@@ -600,6 +603,24 @@ and tc_value env e : exp * lcomp * guard_t =
                                     | _ -> [Util.bvar_to_exp x])) in
                                                        
                      let precedes = Util.ftv Const.precedes_lid kun in
+                     let prev_dec = 
+                        let ct = Util.comp_to_comp_typ c in
+                        match ct.flags |> List.tryFind (function DECREASES _ -> true | _ -> false) with 
+                            | Some (DECREASES dec) -> 
+                               let head, _ = Util.head_and_args_e dec in 
+                               let dec = match head.n with (* The decreases clause is always an expression of type lex_t; promote if it isn't *)
+                                    | Exp_fvar (fv, _) when lid_equals fv.v Const.lexcons_lid -> dec
+                                    | _ -> mk_lex_list [dec] in
+                                let subst = List.map2 (fun b a -> match b, a with 
+                                    | (Inl formal, _), (Inl actual, _) -> Inl (formal.v, Util.btvar_to_typ actual)
+                                    | (Inr formal, _), (Inr actual, _) -> Inr (formal.v, Util.bvar_to_exp actual)
+                                    | _ -> failwith "impossible") bs' actuals in
+                                Util.subst_exp subst dec 
+
+                            | _ -> 
+                                let actual_args = actuals |> filter_types_and_functions in 
+                                mk_lex_list actual_args  in
+
                      let letrecs = letrecs |> List.map (fun (l, t0) -> 
                         let t = Util.alpha_typ t0 in
                         match (Util.compress_typ t).n with 
@@ -614,24 +635,25 @@ and tc_value env e : exp * lcomp * guard_t =
                                             let dec = match head.n with (* The decreases clause is always an expression of type lex_t; promote if it isn't *)
                                                 | Exp_fvar (fv, _) when lid_equals fv.v Const.lexcons_lid -> dec
                                                 | _ -> mk_lex_list [dec] in
-                                            let prev_dec = 
-                                                let subst = List.map2 (fun b a -> match b, a with 
-                                                    | (Inl formal, _), (Inl actual, _) -> Inl (formal.v, Util.btvar_to_typ actual)
-                                                    | (Inr formal, _), (Inr actual, _) -> Inr (formal.v, Util.bvar_to_exp actual)
-                                                    | _ -> failwith "impossible") formals actuals in
-                                                Util.subst_exp subst dec in 
+//                                            let prev_dec = 
+//                                                let subst = List.map2 (fun b a -> match b, a with 
+//                                                    | (Inl formal, _), (Inl actual, _) -> Inl (formal.v, Util.btvar_to_typ actual)
+//                                                    | (Inr formal, _), (Inr actual, _) -> Inr (formal.v, Util.bvar_to_exp actual)
+//                                                    | _ -> failwith "impossible") formals actuals in
+//                                                Util.subst_exp subst dec in 
                                             let dec = 
                                                 let subst = [Inr(x.v, Util.bvar_to_exp y)] in
                                                 Util.subst_exp subst dec in
                                             Syntax.mk_Typ_app(precedes, [varg dec; varg prev_dec]) None r
 
                                         | _ -> (* default measure is lex-tuple of non-type and non-function-typed arguments, in order *)
-                                            let actual_args = actuals |> filter_types_and_functions in 
+//                                            let actual_args = actuals |> filter_types_and_functions in 
                                             let formal_args = (bs@[v_binder y]) |> filter_types_and_functions in
-                                            let lhs, rhs = match formal_args, actual_args with 
-                                                | [f], [a] -> f, a
-                                                | _ -> mk_lex_list formal_args, mk_lex_list actual_args in
-                                            Syntax.mk_Typ_app(precedes, [varg lhs; varg rhs]) None r in
+                                            let lhs = mk_lex_list formal_args in
+//                                            let lhs, rhs = match formal_args, actual_args with 
+//                                                | [f], [a] -> f, a
+//                                                | _ -> mk_lex_list formal_args, mk_lex_list actual_args in
+                                            Syntax.mk_Typ_app(precedes, [varg lhs; varg prev_dec]) None r in
 
                                     let refined_domain = mk_Typ_refine(y, precedes) None r in
                                     let bs = bs@[Inr({x with sort=refined_domain}), imp] in
@@ -793,6 +815,7 @@ and tc_exp env e : exp * lcomp * guard_t =
               tc_args (subst, arg::outargs, arg::arg_rets, comps, g, fvs) rest cres args
 
             | (Inl a, _)::rest, (Inl t, _)::rest' -> (* a concrete type argument *)
+              if debug env Options.Extreme then Util.fprint2 "\tGot a type arg for %s = %s\n" (Print.strBvd a.v) (Print.typ_to_string t);
               let k = Util.subst_kind subst a.sort in 
               fxv_check head env (Inl k) fvs;
               let t, g' = tc_typ_check env t k in
